A few more Depl examples

platform/Depl/examples/Baby.v
@@ -17,3 +17,58 @@ Theorem nadaOk : moduleOk nada.
 Proof.
   depl.
 Qed.
+
+
+(** * Add an easy pure obligation. *)
+
+Definition pure := dmodule "m" {{
+  dfunction "f" [
+    ARGS()
+    PRE Emp
+    POST |^_, (1 + 1 = 2)%nat|
+  ]
+    Return 0
+  end
+}}.
+
+Theorem pureOk : moduleOk pure.
+Proof.
+  depl.
+Qed.
+
+
+(** * Use a contradictory assumption. *)
+
+Definition contra := dmodule "m" {{
+  dfunction "f" [
+    ARGS()
+    PRE |^_, False|
+    POST |^_, (1 + 1 = 3)%nat|
+  ]
+    Return 0
+  end
+}}.
+
+Theorem contraOk : moduleOk contra.
+Proof.
+  depl.
+Qed.
+
+
+(** * Use an assumption about spec variables. *)
+
+Definition assum := dmodule "m" {{
+  dfunction "f" [
+    ARGS()
+    AL "x", AL "y",
+    PRE |^fE, fE "x" = fE "y"|
+    POST |^fE, fE "y" = fE "x"|
+  ]
+    Return 0
+  end
+}}.
+
+Theorem assumOk : moduleOk assum.
+Proof.
+  depl.
+Qed.
